Prove useful property of matcher for le term rules

src/named/Matches.v
@@ -22,7 +22,7 @@ Set Default Proof Mode "Ltac2".
 
 
 (* constructs the union of the two lists viewed as maps,
-   arbitrarily choosing one list when they disagree*)
+   choosing the second list when they disagree*)
 Fixpoint unordered_merge_unsafe {A : eqType} (l1 l2 : named_list A) :=
   match l1 with
   | [::] => l2
@@ -144,14 +144,29 @@ Proof.
   unfold matches_unordered.
   *)
 
-(* Note that 'args' is critical to getting the order of the output subst correct.
-   We assume of the input that FV(pat) is a permutation of args.
- *)
-Definition matches (e pat : exp) (args : list string) : option subst :=
+Definition matches_unordered e pat :=
   (* multiply depth by 2 because each level consumes 1 fuel for exp
      and 1 for its args
    *)
-  do s <- matches_unordered_fuel (exp_depth pat).*2 e pat;
+  matches_unordered_fuel (exp_depth pat).*2 e pat.
+
+
+Definition matches_unordered_sort (t pat : sort) :=
+  match t, pat with
+  | srt n s, srt n_pat s_pat =>
+    if n == n_pat then
+      (* multiply depth by 2 because each level consumes 1 fuel for exp
+     and 1 for its args
+       *)
+      args_match_unordered_fuel (foldl (fun n e => max (exp_depth e) n) 0 s_pat).*2 s s_pat
+    else None
+  end.
+          
+(* Note that 'args' is critical to getting the order of the output subst correct.
+   FV(pat) must be a permutation of args to get a result.
+ *)
+Definition matches (e pat : exp) (args : list string) : option subst :=
+  do s <- matches_unordered e pat;
      s' <- order_subst s args;
      (* this condition can fail because merge doesn't check for conflicts *)
      !e == pat[/s'/];
@@ -216,4 +231,200 @@ Goal
    matches e  (con "foo" [:: con "quox" [::]; var "b"; var "a"]) [::"b";"a"])%string.
   vm_compute.
   reflexivity.
+Qed.
+
+Variant matchable := match_exp (e:exp) | match_sort (s : sort).
+
+Coercion match_exp : exp >-> matchable.
+Coercion match_sort : sort >-> matchable.
+
+(* matching checks only work when the pattern contains all 
+   variables in args. This allows us to use multiple patterns
+   to cover the variables, such as for an equivalence rule
+ *)
+Fixpoint match_all_unordered (l_exp l_pat : list matchable): option subst :=
+  match l_exp, l_pat with
+  | [::], [::] => do ret [::]
+  | (match_exp e)::l'_exp, (match_exp pat)::l'_pat =>
+    do s <- matches_unordered e pat;
+       s' <- match_all_unordered l'_exp l'_pat;
+       ret (unordered_merge_unsafe s s')
+  | (match_sort e)::l'_exp, (match_sort pat)::l'_pat =>
+    do s <- matches_unordered_sort e pat;
+       s' <- match_all_unordered l'_exp l'_pat;
+       ret (unordered_merge_unsafe s s')
+  | _, _ => None
+  end.
+
+Fixpoint check_all (l_exp l_pat : list matchable) s :=
+  match l_exp, l_pat with
+  | [::],[::] => true
+  | (match_exp e)::l'_exp, (match_exp pat)::l'_pat =>
+    (e == pat[/s/]) && (check_all l'_exp l'_pat s)
+  | (match_sort e)::l'_exp, (match_sort pat)::l'_pat =>
+    (e == pat[/s/]) && (check_all l'_exp l'_pat s)
+  | _, _ => false
+end.
+
+Definition match_all l_exp l_pat args :=
+  do s <- match_all_unordered l_exp l_pat;
+     s' <- order_subst s args;
+     (* this condition can fail because merge doesn't check for conflicts *)
+     !check_all l_exp l_pat s';
+     ret s'.
+
+Definition matchable_related s (e p : matchable) : Prop :=
+  match e, p with
+  | match_exp e', match_exp p' => e' = p'[/s/]
+  | match_sort e', match_sort p' => e' = p'[/s/]
+  | _,_ => False
+  end.
+
+Arguments matchable_related s !e !p/.
+
+Lemma check_all_related l lp s
+  : check_all l lp s -> List.Forall2 (matchable_related s) l lp.
+Proof.
+  revert lp; induction l; intro lp; destruct lp; intros; simpl in *;
+    ltac1:(repeat match goal with
+                  | h : matchable |- _=> destruct h
+                  | [h : is_true false |- _] => inversion H
+                  | [|- _ = _] => apply /eqP; assumption
+                  | [|-_ ]=> break; try (constructor; simpl); auto
+                  end).
+Qed.
+
+Lemma match_all_recognizes l lp args s
+  : match_all l lp args = Some s -> List.Forall2 (matchable_related s) l lp.      
+Proof.
+  intro H.
+  apply check_all_related.
+  revert H.
+  unfold match_all.
+  repeat ltac1:(case_match;[|inversion]).
+  intro seq; inversion seq; clear seq; subst.
+  rewrite <-HeqH1.
+  reflexivity.
+Qed.
+
+
+Lemma match_all_args e pat args s
+  : match_all e pat args = Some s ->
+    args = map fst s.
+Proof.
+  unfold match_all.
+  repeat ltac1:(case_match;[|inversion]).
+  ltac1:(inversion); subst.
+  eapply order_subst_args.
+  symmetry; eauto.
+Qed.
+
+(* Designed for the specific case of generating
+   a pair of (potentially) related substitutions *)
+Definition match_all_le l1 lp1 l2 lp2 args : option (subst* subst) :=
+  do s1 <- match_all_unordered l1 lp1;
+     s2 <- match_all_unordered l2 lp2;
+     s1'' <- order_subst (unordered_merge_unsafe s2 s1) args;
+     s2'' <- order_subst (unordered_merge_unsafe s1 s2) args;
+     (* this condition can fail because merge doesn't check for conflicts *)
+     !check_all l1 lp1 s1'';
+     (* this condition can fail because merge doesn't check for conflicts *)
+     !check_all l2 lp2 s2'';
+     ret (s1'',s2'').
+
+Lemma match_all_le_recognizes_l l1 lp1 l2 lp2 args s1 s2
+  : match_all_le l1 lp1 l2 lp2 args = Some (s1,s2) ->
+    List.Forall2 (matchable_related s1) l1 lp1.      
+Proof.
+  intro H.
+  apply check_all_related.
+  revert H.
+  unfold match_all_le.
+  repeat ltac1:(case_match;[|inversion]).
+  intro seq; inversion seq; clear seq; subst.
+  rewrite <-HeqH3.
+  reflexivity.
+Qed.
+
+
+Lemma match_all_le_recognizes_r l1 lp1 l2 lp2 args s1 s2
+  : match_all_le l1 lp1 l2 lp2 args = Some (s1,s2) ->
+    List.Forall2 (matchable_related s2) l2 lp2.      
+Proof.
+  intro H.
+  apply check_all_related.
+  revert H.
+  unfold match_all_le.
+  repeat ltac1:(case_match;[|inversion]).
+  intro seq; inversion seq; clear seq; subst.
+  rewrite <-HeqH4.
+  reflexivity.
+Qed.
+
+
+Lemma match_all_le_args_l l1 lp1 l2 lp2 args s1 s2
+  : match_all_le l1 lp1 l2 lp2 args = Some (s1,s2) ->
+    args = map fst s1.
+Proof.
+  unfold match_all_le.
+  repeat ltac1:(case_match;[|inversion]).
+  ltac1:(inversion); subst.
+  eapply order_subst_args.
+  symmetry; eauto.
+Qed.
+
+
+Lemma match_all_le_args_r l1 lp1 l2 lp2 args s1 s2
+  : match_all_le l1 lp1 l2 lp2 args = Some (s1,s2) ->
+    args = map fst s2.
+Proof.
+  unfold match_all_le.
+  repeat ltac1:(case_match;[|inversion]).
+  ltac1:(inversion); subst.
+  eapply order_subst_args.
+  symmetry; eauto.
+Qed.
+
+Require Import Rule Core.
+
+Definition apply_le_term l n (e1 e2 : exp) (t : sort) : option (subst * subst*ctx) :=
+  do (term_le c pat1 pat2 patt) <- named_list_lookup_err l n;
+  (s1,s2) <- match_all_le [:: e1:matchable]
+                          [:: pat1 : matchable]
+                          [:: t:matchable; e2:matchable]
+                          [:: patt:matchable; pat2:matchable]
+                          (map fst c);
+  ret (s1,s2,c).
+
+Lemma apply_le_term_recognizes l n c e1 e2 t s1 s2 c'
+  : apply_le_term l n e1 e2 t = Some (s1,s2,c') ->
+    le_subst l c c' s1 s2 ->
+    le_term l c t e1 e2.
+Proof.
+  unfold apply_le_term.
+  repeat ltac1:(case_match;[|inversion]).
+  destruct r; 
+    repeat ltac1:(case_match;[|inversion]);
+    try ltac1:(by inversion).
+  ltac1:(break); simpl.
+  intro seq; inversion seq; clear seq; subst.
+  
+  pose HeqH0.
+  symmetry in e3.
+  apply match_all_le_recognizes_l in e3.
+  inversion e3; subst.
+  clear e3 H4.
+  
+  pose HeqH0.
+  symmetry in e3.
+  apply match_all_le_recognizes_r in e3.
+  inversion e3; inversion H5; subst.
+  clear e3 H5 H11.
+
+  simpl in *; subst.
+  intro.
+  symmetry in  HeqH.
+  apply (@named_list_lookup_err_in rule_eqType) in HeqH.  
+  eapply le_term_subst; eauto.
+  eapply le_term_by; eauto.
 Qed.
